cequiv/approx_star_swap.v
@@ -30,46 +30,13 @@
 
 
 Require Export terms_swap.
+Require Export computation_swap.
 Require Export approx_star0.
 
-
-Lemma compute_step_swap_cs1_aux_success_implies {o} :
-  forall can1 can2 l1 l2 bs (t : @NTerm o) u,
-    compute_step_swap_cs1_aux can1 can2 l1 l2 bs t = csuccess u
-    -> {n1 : choice_sequence_name
-       & {n2 : choice_sequence_name
-       & {w : NTerm
-       & can1 = Ncseq n1
-       # can2 = Ncseq n2
-       # l1 = []
-       # l2 = []
-       # bs = [bterm [] w]
-       # u = mk_swap_cs2 n1 n2 w }}}.
-Proof.
-  introv comp.
-  unfold compute_step_swap_cs2 in comp.
-  destruct can1; simpl in comp; ginv.
-  destruct can2; simpl in comp; ginv.
-  destruct l1; simpl in comp; ginv.
-  destruct l2; simpl in comp; ginv.
-  destruct bs as [|b]; ginv.
-  destruct b; simpl in *; ginv.
-  destruct l; simpl in *; ginv.
-  destruct bs; simpl in *; ginv.
-  eexists; eexists; eexists; dands; eauto.
-Qed.
 
 Hint Rewrite @minus0 : slow.
 Hint Rewrite @Nat.add_0_r : slow.
 
-Lemma on_success_csuccess {o} :
-  forall (r : @Comput_Result o) f t,
-    on_success r f = csuccess t
-    -> {u : NTerm & r = csuccess u # t = f u}.
-Proof.
-  introv h.
-  destruct r; simpl in *; ginv; eauto.
-Qed.
 
 Lemma computes_to_val_like_in_max_k_steps_swap_cs1_implies {p} :
   forall lib k n1 n2 n3 v,
@@ -535,106 +502,6 @@ Proof.
   pose proof (change_bvars_alpha_spec t l) as q; simpl in *; repnd; eauto 3 with slow.
 Qed.
 Hint Resolve alpha_eq_change_bvars_alpha : slow.
-
-Lemma cswap_sub_disj {o} :
-  forall a b l k j,
-    disjoint j l
-    -> disjoint j k
-    -> @cswap_sub o (mk_swapping l k) (sw_sub a b j) = sw_sub a b j.
-Proof.
-  introv disja disjb.
-  unfold cswap_sub, sw_sub; rewrite map_map; unfold compose.
-  apply eq_maps; introv i; simpl.
-  applydup disja in i.
-  applydup disjb in i.
-  rewrite swapvar_not_in; tcsp.
-Qed.
-
-Hint Rewrite @osize_cswap : slow.
-
-Lemma implies_alpha_eq_lsubst_aux_sw_sub {o} :
-  forall a b (t u : @NTerm o) l,
-    alpha_eq t u
-    -> alpha_eq (lsubst_aux t (sw_sub a b l)) (lsubst_aux u (sw_sub a b l)).
-Proof.
-  nterm_ind1s t as [v|op bs ind] Case; introv aeq.
-  { inversion aeq; subst; simpl in *; tcsp. }
-  apply alpha_eq_oterm_implies_combine2 in aeq; exrepnd; subst; simpl in *.
-  unfold alpha_eq_bterms in *; repnd.
-
-  apply alpha_eq_oterm_combine; autorewrite with slow; dands; auto.
-  introv i.
-  rewrite <- map_combine in i.
-  apply in_map_iff in i; exrepnd; ginv.
-  destruct a1, a0; simpl in *.
-  applydup aeq0 in i1.
-
-  apply alphaeqbt_eq in i0.
-  apply alphaeqbt_eq; apply alphaeqbt_all; introv.
-  rw @alphaeqbt_all in i0; pose proof (i0 (l ++ l2)) as i0.
-  inversion i0 as [? ? ? ? ? disj lena lenb norep aeq']; subst; clear i0.
-  apply (aeqbt _ vs); auto.
-
-  { allrw disjoint_app_r; repnd; dands; auto;
-      apply disjoint_allvars_lsubst_aux; auto; autorewrite with slow;
-        rw flat_map_map; unfold compose; simpl; autorewrite with slow; eauto 3 with slow. }
-
-  assert (disjoint vs l0) as disj0.
-  { allrw disjoint_app_r; repnd; auto. }
-
-  assert (disjoint vs l1) as disj1.
-  { allrw disjoint_app_r; repnd; auto. }
-
-  assert (disjoint vs l) as disj2.
-  { allrw disjoint_app_r; repnd; auto. }
-
-  assert (disjoint vs (free_vars n)) as disj3.
-  { allrw disjoint_app_r; repnd; auto; introv i j.
-    apply free_vars_subset_allvars in j; apply lenb3 in j; tcsp. }
-
-  assert (disjoint vs (free_vars n0)) as disj4.
-  { allrw disjoint_app_r; repnd; auto; introv i j.
-    apply free_vars_subset_allvars in j; apply lenb in j; tcsp. }
-
-  repeat (rewrite lsubst_aux_cswap_cswap; auto; eauto 2 with slow).
-  autorewrite with slow.
-  apply alphaeq_vs_implies_alphaeq in aeq'; apply alphaeq_eq in aeq'.
-  apply alphaeq_implies_alphaeq_vs; apply alphaeq_eq.
-  repeat (rewrite cswap_sub_disj; eauto 3 with slow).
-
-  assert (subset (remove_nvars l0 l) l) as ssa by (introv i; apply in_remove_nvars in i; tcsp).
-  assert (subset (remove_nvars l1 l) l) as ssb by (introv i; apply in_remove_nvars in i; tcsp).
-  assert (subset (free_vars (cswap (mk_swapping l0 vs) n)) (remove_nvars l0 (free_vars n) ++ vs)) as ssc.
-  { introv i; rewrite free_vars_cswap in i; auto; eauto 2 with slow.
-    apply in_swapbvars in i; exrepnd; subst.
-    apply in_app_iff.
-    destruct (in_deq _ deq_nvar v' l0) as [d|d].
-    { right; apply swapvar_in; auto; eauto 2 with slow.
-      introv xx; apply disj3 in xx; tcsp. }
-    { rewrite swapvar_not_in; tcsp; try (complete (introv xx; apply disj3 in xx; tcsp)).
-      left; apply in_remove_nvars; tcsp. } }
-  assert (subset (free_vars (cswap (mk_swapping l1 vs) n0)) (remove_nvars l1 (free_vars n0) ++ vs)) as ssd.
-  { introv i; rewrite free_vars_cswap in i; auto; eauto 2 with slow.
-    apply in_swapbvars in i; exrepnd; subst.
-    apply in_app_iff.
-    destruct (in_deq _ deq_nvar v' l1) as [d|d].
-    { right; apply swapvar_in; auto; eauto 2 with slow.
-      introv xx; apply disj4 in xx; tcsp. }
-    { rewrite swapvar_not_in; tcsp; try (complete (introv xx; apply disj4 in xx; tcsp)).
-      left; apply in_remove_nvars; tcsp. } }
-
-  erewrite (implies_eq_lsubst_aux_sw_sub _ _ _ (remove_nvars l0 l)); eauto;
-    [|introv i j; apply ssc in j; apply in_remove_nvars; apply in_app_iff in j; dands; auto;
-      allrw in_remove_nvars; repndors; repnd; tcsp; apply disj0 in j; tcsp].
-
-  erewrite (implies_eq_lsubst_aux_sw_sub _ _ _ (remove_nvars l1 l)); eauto;
-    [|introv i j; apply ssd in j; apply in_remove_nvars; apply in_app_iff in j; dands; auto;
-      allrw in_remove_nvars; repndors; repnd; tcsp; apply disj1 in j; tcsp].
-
-  apply in_combine_left_eauto in i1.
-  eapply ind; eauto; autorewrite with slow; eauto 3 with slow.
-Qed.
-Hint Resolve implies_alpha_eq_lsubst_aux_sw_sub : slow.
 
 Lemma lsubst_sw_sub_alpha_eq_aux {o} :
   forall (t : @NTerm o) a b l,
