computation/computation_preserves_utok.v
@@ -2074,6 +2074,29 @@ Proof.
   rewrite ren_utok_lsubst_aux_gen; autorewrite with slow; auto.
 Qed.
 
+Lemma ren_utok_swap_cs_term {o} :
+  forall sw a b (t : @NTerm o),
+    ren_utok (swap_cs_term sw t) a b
+    = swap_cs_term sw (ren_utok t a b).
+Proof.
+  nterm_ind t as [v|op bs ind] Case; introv; simpl; auto.
+  rewrite ren_utok_op_swap_cs_op.
+  f_equal; allrw map_map; unfold compose; apply eq_maps; introv i.
+  destruct x; simpl.
+  erewrite ind; eauto.
+Qed.
+
+Lemma ren_utok_push_swap_cs0 {o} :
+  forall n1 n2 a b (t : @NTerm o),
+    ren_utok (push_swap_cs0 n1 n2 t) a b
+    = push_swap_cs0 n1 n2 (ren_utok t a b).
+Proof.
+  introv; unfold push_swap_cs0, push_swap_cs_sub_term.
+  autorewrite with slow.
+  rewrite ren_utok_lsubst_aux_gen; simpl; autorewrite with slow.
+  rewrite ren_utok_swap_cs_term; auto.
+Qed.
+
 Lemma compute_step_subst_utoken2 {o} :
   forall lib (t u : @NTerm o) v a b,
     nt_wf t
@@ -2273,13 +2296,16 @@ Proof.
               rewrite (not_in_get_utokens_implies_ren_utok_same _ _ a0); eauto 2 with slow.
               rewrite (not_in_get_utokens_implies_ren_utok_same _ _ b0); eauto 2 with slow.
 
-          + allrw @nt_wf_swap_cs1_iff; repndors; exrepnd; subst; simpl in *.
+          + repndors; exrepnd; subst; simpl in *;
+              allrw @nt_wf_swap_cs1_iff;
+              allrw @nt_wf_swap_cs0_iff;
+              exrepnd; subst; simpl in *.
 
             { repeat (destruct bs; simpl in *; ginv).
               inversion wf1; subst; simpl in *; clear wf1.
               repeat (destruct bs1; simpl in *; ginv).
               inversion comp0; subst; simpl in *; clear comp0.
-              apply isnoncan_like_lsubst_aux_is_utok_sub_implies in comp3; eauto with slow;[].
+              apply isnoncan_like_lsubst_aux_is_utok_sub_implies in comp4; eauto with slow;[].
               unfold mk_utoken; rewrite compute_step_swap_cs1_if_isnoncan_like; eauto 3 with slow;[].
               eapply ind in comp1; try (right; left); unfold nobnd; eauto; eauto 3 with slow;
                 [|eapply subset_preserves_not_in_get_utokens_lib; try exact nia
@@ -2295,11 +2321,53 @@ Proof.
               inversion wf1; subst; simpl in *; clear wf1.
               repeat (destruct bs1; simpl in *; ginv).
               inversion comp0; subst; simpl in *; clear comp0.
-              apply (isexc_lsubst_aux_nr_ut_sub lib _ _ b0) in comp2;
+              apply isnoncan_like_lsubst_aux_is_utok_sub_implies in comp4; eauto with slow;[].
+              unfold mk_utoken; rewrite compute_step_swap_cs0_if_isnoncan_like; eauto 3 with slow;[].
+              eapply ind in comp1; try (right; left); unfold nobnd; eauto; eauto 3 with slow;
+                [|eapply subset_preserves_not_in_get_utokens_lib; try exact nia
+                 |eapply subset_preserves_not_in_get_utokens_lib; try exact nib];
+                simpl; autorewrite with slow; eauto 3 with slow.
+              unfold mk_utoken in comp1; allrw; tcsp; fold_terms.
+              rewrite ren_utok_lsubst_aux; auto;[].
+              eapply not_in_get_utokens_lib_implies_not_in_get_utokens;
+                eapply subset_preserves_not_in_get_utokens_lib; try exact nia;
+                  simpl; autorewrite with slow; eauto 3 with slow. }
+
+            { repeat (destruct bs; simpl in *; ginv).
+              inversion wf1; subst; simpl in *; clear wf1.
+              repeat (destruct bs1; simpl in *; ginv).
+              inversion comp0; subst; simpl in *; clear comp0.
+              apply (isexc_lsubst_aux_nr_ut_sub lib _ _ b0) in comp3;
                 try (complete (constructor; simpl; tcsp; intro xx;
                                eapply subset_preserves_not_in_get_utokens_lib; try exact nia;
                                simpl; autorewrite with slow; eauto 3 with slow));[].
-              apply isexc_implies2 in comp2; exrepnd; subst; simpl in *.
+              apply isexc_implies2 in comp3; exrepnd; subst; simpl in *.
+              csunf; simpl; tcsp.
+              unfold ren_utok_op; simpl; tcsp.
+              rewrite map_map; unfold compose.
+              f_equal; f_equal.
+              apply eq_maps; introv i; destruct x0; simpl; f_equal; boolvar; subst; autorewrite with slow; auto.
+              { symmetry; eapply not_in_get_utokens_lib_implies_ren_utok_same;
+                  eapply subset_preserves_not_in_get_utokens_lib; try exact nia;
+                    simpl; autorewrite with slow; eauto 3 with slow.
+                apply subset_app_r; eauto 3 with slow.
+                apply (subsetSingleFlatMap get_utokens_b) in i; simpl in i; auto. }
+              { rewrite ren_utok_lsubst_aux; auto;[].
+                eapply not_in_get_utokens_lib_implies_not_in_get_utokens;
+                  eapply subset_preserves_not_in_get_utokens_lib; try exact nia;
+                    simpl; autorewrite with slow; eauto 3 with slow.
+                apply subset_app_r; eauto 3 with slow.
+                apply (subsetSingleFlatMap get_utokens_b) in i; simpl in i; auto. } }
+
+            { repeat (destruct bs; simpl in *; ginv).
+              inversion wf1; subst; simpl in *; clear wf1.
+              repeat (destruct bs1; simpl in *; ginv).
+              inversion comp0; subst; simpl in *; clear comp0.
+              apply (isexc_lsubst_aux_nr_ut_sub lib _ _ b0) in comp3;
+                try (complete (constructor; simpl; tcsp; intro xx;
+                               eapply subset_preserves_not_in_get_utokens_lib; try exact nia;
+                               simpl; autorewrite with slow; eauto 3 with slow));[].
+              apply isexc_implies2 in comp3; exrepnd; subst; simpl in *.
               csunf; simpl; tcsp.
               unfold ren_utok_op; simpl; tcsp.
               rewrite map_map; unfold compose.
@@ -2849,6 +2917,94 @@ Proof.
                   simpl; autorewrite with slow; eauto 3 with slow;
                     apply subset_app_l; eauto 3 with slow;
                       apply (subsetSingleFlatMap get_utokens_b) in i; simpl in i; auto. } }
+
+            { SSSCase "NSwapCs0".
+              csunf comp; simpl in *.
+              apply compute_step_swap_cs0_success in comp; repndors; exrepnd; subst; simpl in *.
+
+              { repeat (destruct bs; simpl in *; ginv).
+                repeat (destruct bts; simpl in *; ginv).
+                destruct b0, b1; simpl in *.
+                inversion comp2; subst; simpl in *; clear comp2.
+                destruct n; simpl in *; boolvar; ginv.
+                destruct l; simpl in *; ginv.
+                csunf; simpl.
+                unfold ren_utok_op; simpl; fold_terms.
+                rewrite ren_utok_push_swap_cs0.
+                rewrite ren_utok_lsubst_aux_gen; simpl; unfold ren_utok_op; simpl; boolvar; GC; tcsp.
+                erewrite not_in_get_utokens_lib_implies_ren_utok_same; tcsp.
+                eapply subset_preserves_not_in_get_utokens_lib; try exact nia;
+                  simpl; autorewrite with slow; eauto 3 with slow;
+                    apply subset_app_l; eauto 3 with slow;
+                      apply (subsetSingleFlatMap get_utokens_b) in i; simpl in i; auto. }
+
+              { destruct bs; simpl in *; ginv.
+                destruct b0; simpl in *.
+                inversion comp0; subst; simpl in *; clear comp0.
+                destruct n; simpl in *; boolvar; ginv.
+                csunf; unfold ren_utok_op; simpl.
+                rewrite map_map; unfold compose.
+                f_equal; f_equal; apply eq_maps; introv i; destruct x; simpl; f_equal; simpl.
+                boolvar; subst; tcsp; autorewrite with slow; fold_terms.
+                { erewrite not_in_get_utokens_lib_implies_ren_utok_same; tcsp.
+                  eapply subset_preserves_not_in_get_utokens_lib; try exact nia.
+                  simpl; autorewrite with slow; eauto 3 with slow.
+                  apply subset_app_l; apply subset_app_r.
+                  apply (subsetSingleFlatMap get_utokens_b) in i; simpl in i; auto. }
+                { rewrite ren_utok_lsubst_aux_gen; simpl; unfold ren_utok_op; simpl; boolvar; GC; tcsp.
+                  erewrite not_in_get_utokens_lib_implies_ren_utok_same; tcsp.
+                  eapply subset_preserves_not_in_get_utokens_lib; try exact nia.
+                  simpl; autorewrite with slow; eauto 3 with slow.
+                  apply subset_app_l; apply subset_app_r.
+                  apply (subsetSingleFlatMap get_utokens_b) in i; simpl in i; auto. } }
+
+              { destruct bs; simpl in *; ginv.
+                destruct b0; simpl in *.
+                inversion comp0; subst; simpl in *; clear comp0.
+                apply nt_wf_swap_cs0_iff in wf; exrepnd.
+                repeat (destruct bs; simpl in *; ginv).
+                destruct b1; inversion wf1; subst; simpl in *; clear wf1.
+                destruct b0; simpl in *; boolvar; ginv.
+                { unfold mk_utoken in *; ginv; simpl in *; fold_terms.
+                  inversion comp3; simpl in *; tcsp. }
+                unfold ren_utok_op; simpl.
+                rewrite ren_utok_match_can_as.
+                rewrite subst_aux_oterm; simpl.
+                unfold subst_bterm_aux; simpl.
+                rewrite compute_step_swap_cs0_if_isnoncan_like; eauto 3 with slow;[].
+                rewrite <- subst_aux_oterm2 in comp2.
+                eapply ind in comp2; try (right; left); try reflexivity; auto;
+                  [|
+                   |eapply subset_preserves_not_in_get_utokens_lib; try exact nia;
+                    simpl; autorewrite with slow; eauto 3 with slow
+                   |eapply subset_preserves_not_in_get_utokens_lib; try exact nib;
+                    simpl; autorewrite with slow; eauto 3 with slow]; eauto 3 with slow;[].
+                rewrite subst_aux_oterm in comp2; simpl in comp2.
+                unfold subst_bterm_aux in *; allrw; simpl.
+                f_equal.
+                rewrite ren_utok_lsubst_aux_gen; simpl.
+                unfold ren_utok_op; simpl; simpl; boolvar; GC; tcsp.
+                erewrite (not_in_get_utokens_lib_implies_ren_utok_same _ _ _ c); tcsp;
+                  try (complete (eapply subset_preserves_not_in_get_utokens_lib; try exact nia;
+                                 simpl; autorewrite with slow; eauto 3 with slow)); fold_terms.
+                f_equal; f_equal.
+                { destruct can2; simpl; auto; boolvar; subst; tcsp.
+                  destruct nia; apply in_get_utokens_implies_in_get_utokens_lib; simpl; autorewrite with slow; tcsp. }
+                rewrite map_map; unfold compose.
+                apply eq_maps; introv i; destruct x; simpl; f_equal.
+                boolvar; subst; tcsp; autorewrite with slow; fold_terms.
+                { erewrite not_in_get_utokens_lib_implies_ren_utok_same; tcsp.
+                  eapply subset_preserves_not_in_get_utokens_lib; try exact nia.
+                  simpl; autorewrite with slow; eauto 3 with slow.
+                  apply subset_app_r; apply subset_app_l.
+                  apply (subsetSingleFlatMap get_utokens_b) in i; simpl in i; auto. }
+                { rewrite ren_utok_lsubst_aux_gen; simpl; unfold ren_utok_op; simpl; boolvar; GC; tcsp.
+                  erewrite not_in_get_utokens_lib_implies_ren_utok_same; tcsp.
+                  eapply subset_preserves_not_in_get_utokens_lib; try exact nia.
+                  simpl; autorewrite with slow; eauto 3 with slow.
+                  apply subset_app_r; apply subset_app_l.
+                  apply (subsetSingleFlatMap get_utokens_b) in i; simpl in i; auto. } }
+            }
 
             { SSSCase "NLDepth".
               csunf comp; simpl in *; ginv. }
