terms/opid.v
@@ -475,6 +475,7 @@ Inductive NonCanonicalOp : Set :=
  | NParallel  : NonCanonicalOp
  | NSwapCs1   : NonCanonicalOp
  | NSwapCs2   : SwapCsNfo -> NonCanonicalOp
+ | NSwapCs0   : NonCanonicalOp
 (* | NSwapCs    : NonCanonicalOp*)
  | NLDepth    : NonCanonicalOp
  | NLastCs    : NonCanonicalOp
@@ -508,6 +509,7 @@ Definition OpBindingsNCan (nc : NonCanonicalOp) : opsign :=
   | NParallel    => [0,0]
   | NSwapCs1     => [0,0,0]
   | NSwapCs2 _   => [0]
+  | NSwapCs0     => [0,0,0]
 (*  | NSwapCs      => [0,0,0]*)
   | NLDepth      => []
   | NLastCs      => [0,0]
@@ -631,6 +633,7 @@ Tactic Notation "dopid_noncan" ident(onc) ident(c) :=
   | Case_aux c "NParallel"
   | Case_aux c "NSwapCs1"
   | Case_aux c "NSwapCs2"
+  | Case_aux c "NSwapCs0"
 (*  | Case_aux c "NSwapCs"*)
   | Case_aux c "NLDepth"
   | Case_aux c "NLastCs"
